theory/ComplexityNat.dfy
@@ -1,6 +1,9 @@
 include "./math/ExpNat.dfy"
+include "./math/Factorial.dfy"
 include "./math/FloorCeil.dfy"
 include "./math/LemFunction.dfy"
+include "./math/LogNat.dfy"
+include "./math/SqrtNat.dfy"
 include "./math/TypeR0.dfy"
 include "./ComplexityR0.dfy"
 
@@ -10,10 +13,15 @@ include "./ComplexityR0.dfy"
 
 module ComplexityNat { 
   import opened ExpNat
+  import opened Factorial  
   import opened FloorCeil   
   import opened LemFunction
+  import opened LogNat
+  import opened SqrtNat
   import opened TypeR0 
   import CR0 = ComplexityR0
+
+  /* Big O */
 
   ghost predicate bigO(f:nat->nat, g:nat->nat)
   { 
@@ -35,139 +43,95 @@ module ComplexityNat {
     exists k:nat :: bigO(f, n => pow(n,k))
   }
 
-  /**************************************************************************
-    Mapping of results between unlifted and lifted functions
-  **************************************************************************/
+  /* Big Ω */
 
-  // If we prove f ∈ O(g) for f,g:nat->nat then we can extend
-  // the result for the lifted versions f',g':nat->R0.
-  lemma lem_bigOtoBigOR0(f:nat->nat, g:nat->nat)  
-    requires bigO(f, g) 
-    ensures  CR0.bigO(liftToR0(f), liftToR0(g))
-  {    
-    var c:nat, n0:nat :| bigOfrom(c, n0, f, g);  
-    assert forall n:nat :: 0 <= n0 <= n ==> f(n) <= c*g(n);
+  ghost predicate bigOmega(f:nat->nat, g:nat->nat)
+  { 
+    exists c:nat, n0:nat :: bigOmegaFrom(c, n0, f, g) 
+  }
 
-    assert forall n:nat :: liftToR0(f)(n) == f(n) as R0;
-    assert forall n:nat :: liftToR0(g)(n) == g(n) as R0;
+  ghost predicate bigOmegaFrom(c:nat, n0:nat, f:nat->nat, g:nat->nat)
+  {
+    forall n:nat :: 0 <= n0 <= n ==> c*g(n) <= f(n)
+  }
 
-    var c':R0 := c as R0; // just view c:nat as a R0 number
-    assert forall n:nat :: 0 <= n0 <= n ==> liftToR0(f)(n) <= c'*liftToR0(g)(n); 
-    assert CR0.bigOfrom(c', n0, liftToR0(f), liftToR0(g));
+  ghost predicate tIsBigOmega(n:nat, t:nat, g:nat->nat)
+  { 
+    exists f:nat->nat :: f(n) <= t && bigOmega(f, g)
+  }
+
+  /* Big Θ */
+
+  ghost predicate bigTheta1(f:nat->nat, g:nat->nat)
+  { 
+    bigOmega(f, g) && bigO(f, g) 
+  }
+
+  ghost predicate bigTheta2(f:nat->nat, g:nat->nat)
+  { 
+    exists c1:nat, c2:nat, n0:nat :: bigThetaFrom(c1, c2, n0, f, g) 
+  }
+
+  ghost predicate bigThetaFrom(c1:nat, c2:nat, n0:nat, f:nat->nat, g:nat->nat)
+  {
+    forall n:nat :: 0 <= n0 <= n ==> c1*g(n) <= f(n) <= c2*g(n)  
   }
   
-  // If we prove f' ∈ O(g') for the lifted versions of f,g:nat->nat
-  // then we can get back the result
-  lemma lem_bigOR0toBigO(f:nat->nat, g:nat->nat)  
-    requires CR0.bigO(liftToR0(f), liftToR0(g))
-    ensures  bigO(f, g)
-  { 
-    var c:R0, n0:nat :| CR0.bigOfrom(c, n0, liftToR0(f), liftToR0(g));
-    assert forall n:nat :: 0 <= n0 <= n ==> liftToR0(f)(n) <= c*liftToR0(g)(n);
-    
-    assert forall n:nat :: liftToR0(f)(n) == f(n) as R0;
-    assert forall n:nat :: liftToR0(g)(n) == g(n) as R0;
+  /* Common growth rates */
 
-    var c':nat := ceil(c);  // c may be non-integer, so we bound with it's ceil
-    assert c <= c' as R0;
-    assert forall n:nat :: c*liftToR0(g)(n) <= (c' as R0)*liftToR0(g)(n);
-    assert forall n:nat :: 0 <= n0 <= n ==> f(n) <= c'*g(n); 
-    assert bigOfrom(c', n0, f, g);
+  ghost function constGrowth() : nat->nat
+  {   
+    n => 1
   }
 
-  /**************************************************************************
-    Basic O properties
-  **************************************************************************/
-  // Each result is proved in the lifted domain nat->R0
-  // and then casted back to nat->nat 
-
-  // Reflexivity
-  // f ∈ O(f)
-  lemma lem_bigO_refl(f:nat->nat)  
-    ensures bigO(f, f) 
-  {  
-    var f':nat->R0 := liftToR0(f);
-    assert CR0.bigO(f', f')
-      by { CR0.lem_bigO_refl(f'); }
-    lem_bigOR0toBigO(f, f);
+  ghost function logGrowth() : nat->nat
+  {   
+    n => if n>0 then log2(n) else 0
   }
 
-  // If f ∈ O(g) and a>0 then a*f ∈ O(g)
-  lemma lem_bigO_constFactor(f:nat->nat, g:nat->nat, a:nat)  
-    requires bigO(f, g) 
-    requires a > 0
-    ensures  bigO(n => a*f(n), g) 
-  {  
-    var f':nat->R0 := liftToR0(f);
-    var g':nat->R0 := liftToR0(g); 
-    var a':R0 := a as R0; 
-    assert CR0.bigO(f', g') 
-      by { lem_bigOtoBigOR0(f, g); }
-    assert CR0.bigO(n => a'*f'(n), g')  
-      by { CR0.lem_bigO_constFactor(f', g', a'); }
-    lem_bigOR0toBigO(n => a*f(n), g)
-      by { lem_funExt(liftToR0(n => a*f(n)), n => a'*f'(n)); }
-  } 
-
-  // If f1 ∈ O(g1) and f2 ∈ O(g2) then f1+f2 ∈ O(g1+g2)
-  lemma lem_bigO_sum(f1:nat->nat, g1:nat->nat, f2:nat->nat, g2:nat->nat)  
-    requires bigO(f1, g1) 
-    requires bigO(f2, g2) 
-    ensures  bigO(n => f1(n)+f2(n), n => g1(n)+g2(n)) 
-  {  
-    var f1':nat->R0 := liftToR0(f1);
-    var f2':nat->R0 := liftToR0(f2);
-    var g1':nat->R0 := liftToR0(g1); 
-    var g2':nat->R0 := liftToR0(g2); 
-    assert CR0.bigO(f1', g1') 
-      by { lem_bigOtoBigOR0(f1, g1); }
-    assert CR0.bigO(f2', g2') 
-      by { lem_bigOtoBigOR0(f2, g2); } 
-    assert CR0.bigO(n => f1'(n)+f2'(n), n => g1'(n)+g2'(n))  
-      by { CR0.lem_bigO_sum(f1', g1', f2', g2'); }
-    lem_funExt(liftToR0(n => f1(n)+f2(n)), n => f1'(n)+f2'(n));
-    lem_funExt(liftToR0(n => g1(n)+g2(n)), n => g1'(n)+g2'(n));  
-    lem_bigOR0toBigO(n => f1(n)+f2(n), n => g1(n)+g2(n));     
+  ghost function logGrowth2() : nat->nat
+  {   
+    n => log2(n+1)
   }
 
-  // If f1 ∈ O(g1) and f2 ∈ O(g2) then f1*f2 ∈ O(g1*g2)
-  lemma lem_bigO_prod(f1:nat->nat, g1:nat->nat, f2:nat->nat, g2:nat->nat)  
-    requires bigO(f1, g1) 
-    requires bigO(f2, g2) 
-    ensures  bigO(n => f1(n)*f2(n), n => g1(n)*g2(n))  
-  {  
-    var f1':nat->R0 := liftToR0(f1);
-    var f2':nat->R0 := liftToR0(f2);
-    var g1':nat->R0 := liftToR0(g1); 
-    var g2':nat->R0 := liftToR0(g2);  
-    assert A: CR0.bigO(f1', g1') 
-      by { lem_bigOtoBigOR0(f1, g1); }
-    assert B: CR0.bigO(f2', g2') 
-      by { lem_bigOtoBigOR0(f2, g2); } 
-    assert CR0.bigO(n => f1'(n)*f2'(n), n => g1'(n)*g2'(n))  
-      by { reveal A, B; CR0.lem_bigO_prod(f1', g1', f2', g2'); }
-    lem_funExt(liftToR0(n => f1(n)*f2(n)), n => f1'(n)*f2'(n));
-    lem_funExt(liftToR0(n => g1(n)*g2(n)), n => g1'(n)*g2'(n));
-    lem_bigOR0toBigO(n => f1(n)*f2(n), n => g1(n)*g2(n));
-  }   
+  ghost function sqrtGrowth() : nat->nat
+  {   
+    n => sqrt(n)
+  }
 
-  // Transitivity
-  // If f ∈ O(g) and g ∈ O(h) then f ∈ O(h)
-  lemma lem_bigO_trans(f:nat->nat, g:nat->nat, h:nat->nat)  
-    requires bigO(f, g)
-    requires bigO(g, h)
-    ensures  bigO(f, h) 
-  {  
-    var f':nat->R0 := liftToR0(f);
-    var g':nat->R0 := liftToR0(g);  
-    var h':nat->R0 := liftToR0(h);  
-    assert CR0.bigO(f', g') 
-      by { lem_bigOtoBigOR0(f, g); }
-    assert CR0.bigO(g', h') 
-      by { lem_bigOtoBigOR0(g, h); }
-    assert CR0.bigO(f', h')  
-      by { CR0.lem_bigO_trans(f', g', h'); }
-    lem_bigOR0toBigO(f, h);
+  ghost function linGrowth() : nat->nat
+  {   
+    n => pow(n,1)
+  }
+
+  ghost function quadGrowth() : nat->nat
+  {   
+    n => pow(n,2)
+  }
+
+  ghost function cubicGrowth() : nat->nat
+  {   
+    n => pow(n,3)
+  }
+
+  ghost function polyGrowth(k:nat) : nat->nat
+  {   
+    n => pow(n,k)
+  }
+
+  ghost function expGrowth() : nat->nat
+  {   
+    n => pow(2,n)
+  }
+
+  ghost function facGrowth() : nat->nat
+  {   
+    n => fac(n)
+  }
+
+  ghost function dexpGrowth() : nat->nat
+  {   
+    n => pow(2,pow(2,n))
   }
 
 }
