analysisByF/breakConstBT.dfy
@@ -1,8 +1,6 @@
 include "../theory/ComplexityNat.dfy"
-include "../theory/GrowthRatesNat.dfy"
 
 import opened ComplexityNat
-import opened GrowthRatesNat
 
 ghost function f(N:nat) : nat
 {
