analysisByMM/quad.dfy
@@ -2,14 +2,12 @@ include "../theory/math/ExpReal.dfy"
 include "../theory/math/LemFunction.dfy"
 include "../theory/math/TypeR0.dfy"
 include "../theory/ComplexityR0.dfy"
-include "../theory/GrowthRatesR0.dfy"
 include "../theory/MasterLR.dfy"
 
 import opened ExpReal
 import opened LemFunction
 import opened TypeR0
 import opened ComplexityR0
-import opened GrowthRatesR0
 import opened MasterLR
 
 method quad(N:nat)
