analysisBySum/breakLinWT.dfy
@@ -1,12 +1,10 @@
 include "../theory/math/ExpNat.dfy"
 include "../theory/math/SumInt.dfy"
 include "../theory/ComplexityNat.dfy"
-include "../theory/GrowthRatesNat.dfy"
 
 import opened ExpNat
 import opened SumInt
 import opened ComplexityNat
-import opened GrowthRatesNat
 
 ghost function f(N:nat) : nat
 {
@@ -18,7 +16,7 @@ method breakLinWT(N:nat, P:nat->bool)
   ensures t == f(N)
   ensures tIsBigO(N, t, linGrowth())
 {
-  assume {:axiom} forall i :: 0 <= i <= N ==> !P(i);  // worst case
+  assume {:axiom} forall i :: 0 <= i < N ==> !P(i);  // worst case
   var i; reveal sum(); 
   i, t := 0, 0;
   while i != N
