analysisBySum/quadNM.dfy
@@ -1,12 +1,10 @@
 include "../theory/math/ExpNat.dfy"
 include "../theory/math/SumInt.dfy"
 include "../theory/ComplexityNat.dfy"
-include "../theory/GrowthRatesNat.dfy"
 
 import opened ExpNat
 import opened SumInt
 import opened ComplexityNat
-import opened GrowthRatesNat
 
 ghost function f(N:nat, M:nat) : nat
 {
