theory/LemComplexityNat.dfy
@@ -1,0 +1,226 @@
+include "./math/ExpNat.dfy"
+include "./math/FloorCeil.dfy"
+include "./math/LemBoundsNat.dfy"
+include "./math/LemFunction.dfy"
+include "./math/TypeR0.dfy"
+include "./ComplexityNat.dfy"
+include "./ComplexityR0.dfy"
+include "./LemComplexity.dfy"
+include "./LemComplexityR0.dfy"
+
+/**************************************************************************
+  Lemmas about complexity of non-negative integer functions
+**************************************************************************/
+
+module LemComplexityNat { 
+  import opened ExpNat
+  import opened FloorCeil   
+  import opened LemBoundsNat
+  import opened LemFunction
+  import opened TypeR0 
+  import opened ComplexityNat
+  import CR0 = ComplexityR0
+  import opened LemComplexity
+  import LCR0 = LemComplexityR0
+
+  /* BigTheta1 and bigTheta2 are equivalent definitions of Big Θ */
+ 
+  lemma lem_bigTheta_def1EQLdef2(f:nat->nat, g:nat->nat)  
+    ensures bigTheta1(f, g) <==> bigTheta2(f, g)
+  {
+    var f':nat->R0 := liftToR0(f);
+    var g':nat->R0 := liftToR0(g); 
+    
+    assert bigTheta1(f, g) ==> bigTheta2(f, g) by {
+      assume {:axiom} bigTheta1(f, g);
+      assert CR0.bigTheta1(f', g')
+        by { lem_bigT1toBigT1R0(f, g); }
+      assert CR0.bigTheta1(f', g') ==> CR0.bigTheta2(f', g')
+        by { LCR0.lem_bigTheta_def1IMPLdef2(f', g'); }
+      assert CR0.bigTheta2(f', g');
+      assert bigTheta2(f, g)
+        by { lem_bigT2R0toBigT2(f, g); }  
+    }
+
+    assert bigTheta2(f, g) ==> bigTheta1(f, g) by {
+      assume {:axiom} bigTheta2(f, g);
+      assert CR0.bigTheta2(f', g')
+        by { lem_bigT2toBigT2R0(f, g); }
+      assert CR0.bigTheta2(f', g') ==> CR0.bigTheta1(f', g')
+        by { LCR0.lem_bigTheta_def2IMPLdef1(f', g'); }
+      assert CR0.bigTheta1(f', g');
+      assert bigTheta1(f, g)
+        by { lem_bigT1R0toBigT1(f, g); }  
+    }
+  }
+
+  /* Big O basic properties */
+  // Each result is proved in the lifted domain nat->R0
+  // and then casted back to nat->nat 
+
+  // Reflexivity
+  // f ∈ O(f)
+  lemma lem_bigO_refl(f:nat->nat)  
+    ensures bigO(f, f) 
+  {  
+    var f':nat->R0 := liftToR0(f);
+    assert CR0.bigO(f', f')
+      by { LCR0.lem_bigO_refl(f'); }
+    lem_bigOR0toBigO(f, f);
+  }
+
+  // If f ∈ O(g) and a>0 then a*f ∈ O(g)
+  lemma lem_bigO_constFactor(f:nat->nat, g:nat->nat, a:nat)  
+    requires bigO(f, g) 
+    requires a > 0
+    ensures  bigO(n => a*f(n), g) 
+  {  
+    var f':nat->R0 := liftToR0(f);
+    var g':nat->R0 := liftToR0(g); 
+    var a':R0 := a as R0; 
+    assert CR0.bigO(f', g') 
+      by { lem_bigOtoBigOR0(f, g); }
+    assert CR0.bigO(n => a'*f'(n), g')  
+      by { LCR0.lem_bigO_constFactor(f', g', a'); }
+    lem_bigOR0toBigO(n => a*f(n), g)
+      by { lem_funExt(liftToR0(n => a*f(n)), n => a'*f'(n)); }
+  } 
+
+  // If f1 ∈ O(g1) and f2 ∈ O(g2) then f1+f2 ∈ O(g1+g2)
+  lemma lem_bigO_sum(f1:nat->nat, g1:nat->nat, f2:nat->nat, g2:nat->nat)  
+    requires bigO(f1, g1) 
+    requires bigO(f2, g2) 
+    ensures  bigO(n => f1(n)+f2(n), n => g1(n)+g2(n)) 
+  {  
+    var f1':nat->R0 := liftToR0(f1);
+    var f2':nat->R0 := liftToR0(f2);
+    var g1':nat->R0 := liftToR0(g1); 
+    var g2':nat->R0 := liftToR0(g2); 
+    assert CR0.bigO(f1', g1') 
+      by { lem_bigOtoBigOR0(f1, g1); }
+    assert CR0.bigO(f2', g2') 
+      by { lem_bigOtoBigOR0(f2, g2); } 
+    assert CR0.bigO(n => f1'(n)+f2'(n), n => g1'(n)+g2'(n))  
+      by { LCR0.lem_bigO_sum(f1', g1', f2', g2'); }
+    lem_funExt(liftToR0(n => f1(n)+f2(n)), n => f1'(n)+f2'(n));
+    lem_funExt(liftToR0(n => g1(n)+g2(n)), n => g1'(n)+g2'(n));  
+    lem_bigOR0toBigO(n => f1(n)+f2(n), n => g1(n)+g2(n));     
+  }
+
+  // If f1 ∈ O(g1) and f2 ∈ O(g2) then f1*f2 ∈ O(g1*g2)
+  lemma lem_bigO_prod(f1:nat->nat, g1:nat->nat, f2:nat->nat, g2:nat->nat)  
+    requires bigO(f1, g1) 
+    requires bigO(f2, g2) 
+    ensures  bigO(n => f1(n)*f2(n), n => g1(n)*g2(n))  
+  {  
+    var f1':nat->R0 := liftToR0(f1);
+    var f2':nat->R0 := liftToR0(f2);
+    var g1':nat->R0 := liftToR0(g1); 
+    var g2':nat->R0 := liftToR0(g2);  
+    assert A: CR0.bigO(f1', g1') 
+      by { lem_bigOtoBigOR0(f1, g1); }
+    assert B: CR0.bigO(f2', g2') 
+      by { lem_bigOtoBigOR0(f2, g2); } 
+    assert CR0.bigO(n => f1'(n)*f2'(n), n => g1'(n)*g2'(n))  
+      by { reveal A, B; LCR0.lem_bigO_prod(f1', g1', f2', g2'); }
+    lem_funExt(liftToR0(n => f1(n)*f2(n)), n => f1'(n)*f2'(n));
+    lem_funExt(liftToR0(n => g1(n)*g2(n)), n => g1'(n)*g2'(n));
+    lem_bigOR0toBigO(n => f1(n)*f2(n), n => g1(n)*g2(n));
+  }   
+
+  // Transitivity
+  // If f ∈ O(g) and g ∈ O(h) then f ∈ O(h)
+  lemma lem_bigO_trans(f:nat->nat, g:nat->nat, h:nat->nat)  
+    requires bigO(f, g)
+    requires bigO(g, h)
+    ensures  bigO(f, h) 
+  {  
+    var f':nat->R0 := liftToR0(f);
+    var g':nat->R0 := liftToR0(g);  
+    var h':nat->R0 := liftToR0(h);  
+    assert CR0.bigO(f', g') 
+      by { lem_bigOtoBigOR0(f, g); }
+    assert CR0.bigO(g', h') 
+      by { lem_bigOtoBigOR0(g, h); }
+    assert CR0.bigO(f', h')  
+      by { LCR0.lem_bigO_trans(f', g', h'); }
+    lem_bigOR0toBigO(f, h);
+  }
+
+  /* Common growth rates comparison */
+  
+  // log2(n) ∈ O(n) 
+  lemma lem_bigO_logBigOlin()
+    ensures bigO(logGrowth(), linGrowth()) 
+  { 
+    // we show that c=1 and n0=1
+    var c:nat, n0:nat := 1, 1;
+    forall n:nat | 0 <= n0 <= n
+      ensures logGrowth()(n) <= c*linGrowth()(n)
+    {
+      reveal pow();
+      lem_log2nLEQnMinus1(n);
+      assert logGrowth()(n) <= c*linGrowth()(n);
+    }
+    assert bigOfrom(c, n0, logGrowth(), linGrowth());
+  }
+
+  // log2(n+1) ∈ O(n) 
+  lemma lem_bigO_logBigOlinV2()
+    ensures bigO(logGrowth2(), linGrowth())
+  { 
+    // we show that c=1 and n0=1
+    var c:nat, n0:nat := 1, 1;
+    forall n:nat | 0 <= n0 <= n
+      ensures logGrowth2()(n) <= c*linGrowth()(n)
+    {
+      reveal pow();
+      lem_log2nPlus1LEQn(n);
+      assert logGrowth2()(n) <= c*linGrowth()(n);
+    }
+    assert bigOfrom(c, n0, logGrowth2(), linGrowth());
+  }
+
+  // n ∈ O(n^2) 
+  lemma lem_bigO_linBigOquad()
+    ensures bigO(linGrowth(), quadGrowth()) 
+  { 
+    // we show that c=1 and n0=0
+    var c:nat, n0:nat := 1, 0;
+    forall n:nat | 0 <= n0 <= n
+      ensures linGrowth()(n) <= c*quadGrowth()(n)
+    {
+      reveal pow();
+      lem_nLQpown2(n);
+      assert linGrowth()(n) <= c*quadGrowth()(n);
+    }
+    assert bigOfrom(c, n0, linGrowth(), quadGrowth());
+  }
+
+  // n^2 ∈ O(2^n)  
+  lemma lem_bigO_quadBigOexp()
+    ensures bigO(quadGrowth(), expGrowth()) 
+  { 
+    // we show that c=1 and n0=4
+    var c:nat, n0:nat := 1, 4;
+    forall n:nat | 0 <= n0 <= n
+      ensures quadGrowth()(n) <= c*expGrowth()(n)
+    {
+      reveal pow();
+      lem_pown2LQpow2n(n);
+      assert quadGrowth()(n) <= c*expGrowth()(n);
+    }
+    assert bigOfrom(c, n0, quadGrowth(), expGrowth());
+  }
+
+  // n ∈ O(2^n)  
+  // Follows from transitivity of n ∈ O(n^2) and n^2 ∈ O(2^n)  
+  lemma lem_bigO_linBigOexp()
+    ensures bigO(linGrowth(), expGrowth()) 
+  { 
+    assert bigO(linGrowth(), quadGrowth()) by { lem_bigO_linBigOquad(); }
+    assert bigO(quadGrowth(), expGrowth()) by { lem_bigO_quadBigOexp(); }
+    lem_bigO_trans(linGrowth(), quadGrowth(), expGrowth());
+  }
+
+}
