theory/LemComplexityR0.dfy
@@ -1,0 +1,198 @@
+include "./math/ExpNat.dfy"
+include "./math/FloorCeil.dfy"
+include "./math/LemBoundsNat.dfy"
+include "./math/LemFunction.dfy"
+include "./math/LogNat.dfy"
+include "./math/TypeR0.dfy"
+include "./ComplexityNat.dfy"
+include "./ComplexityR0.dfy"
+include "./LemComplexity.dfy"
+
+/**************************************************************************
+  Lemmas about complexity of lifted functions
+**************************************************************************/
+
+module LemComplexityR0 { 
+  import opened ExpNat
+  import opened FloorCeil   
+  import opened LemBoundsNat
+  import opened LemFunction
+  import opened LogNat  
+  import opened TypeR0 
+  import opened ComplexityR0
+
+  /* BigTheta1 and bigTheta2 are equivalent definitions of Big Θ */
+  
+  lemma lem_bigTheta_def1EQLdef2(f:nat->R0, g:nat->R0)  
+    ensures bigTheta1(f, g) <==> bigTheta2(f, g)
+  {
+    assert bigTheta1(f, g) ==> bigTheta2(f, g) by {
+      assume {:axiom} bigTheta1(f, g);
+      lem_bigTheta_def1IMPLdef2(f, g);
+    }
+    assert bigTheta2(f, g) ==> bigTheta1(f, g) by {
+      assume {:axiom} bigTheta2(f, g);
+      lem_bigTheta_def2IMPLdef1(f, g);
+    }
+  }
+
+  lemma lem_bigTheta_def1IMPLdef2(f:nat->R0, g:nat->R0)  
+    requires bigTheta1(f, g) 
+    ensures  bigTheta2(f, g)
+  {
+    var c1:R0, n0_1:nat :| bigOmegaFrom(c1, n0_1, f, g) ; 
+    assert H1: forall n:nat :: 0 <= n0_1 <= n ==> c1*g(n) <= f(n);
+
+    var c2:R0, n0_2:nat :| bigOfrom(c2, n0_2, f, g) ; 
+    assert H2: forall n:nat :: 0 <= n0_2 <= n ==> f(n) <= c2*g(n);
+
+    var n0 := n0_1 + n0_2;
+    forall n:nat | 0 <= n0 <= n
+      ensures c1*g(n) <= f(n) <= c2*g(n)
+    {
+      assert c1*g(n) <= f(n) by { reveal H1; }
+      assert f(n) <= c2*g(n) by { reveal H2; }
+    }
+    assert bigThetaFrom(c1, c2, n0, f, g);
+  }
+
+  lemma lem_bigTheta_def2IMPLdef1(f:nat->R0, g:nat->R0)  
+    requires bigTheta2(f, g) 
+    ensures  bigTheta1(f, g)
+  {
+    var c1:R0, c2:R0, n0:nat :| bigThetaFrom(c1, c2, n0, f, g); 
+    assert H: forall n:nat :: 0 <= n0 <= n ==> c1*g(n) <= f(n) <= c2*g(n);
+
+    assert A: bigO(f, g) by {
+      forall n:nat | 0 <= n0 <= n
+        ensures f(n) <= c2*g(n)
+      {
+        assert f(n) <= c2*g(n) by { reveal H; }
+      }
+      assert bigOfrom(c2, n0, f, g);
+    }
+    assert B: bigOmega(f, g) by {
+      forall n:nat | 0 <= n0 <= n
+        ensures c1*g(n) <= f(n)
+      {
+        assert c1*g(n) <= f(n) by { reveal H; }
+      }
+      assert bigOmegaFrom(c1, n0, f, g);
+    }
+    
+    assert bigO(f, g) && bigOmega(f, g) by { reveal A, B; }
+  }      
+
+  /* Big O basic properties */
+
+  // Reflexivity
+  // f ∈ O(f)
+  lemma lem_bigO_refl(f:nat->R0)  
+    ensures bigO(f, f) 
+  {  
+    // we show that c=1.0 and n0=0
+    assert forall n:nat :: 0 <= 0 <= n ==> f(n) <= 1.0*f(n);
+    assert bigOfrom(1.0, 0, f, f);
+  }
+
+  // If f ∈ O(g) and a>0 then a*f ∈ O(g)
+  lemma lem_bigO_constFactor(f:nat->R0, g:nat->R0, a:R0)  
+    requires bigO(f, g) 
+    requires a > 0.0 
+    ensures  bigO(n => a*f(n), g) 
+  {  
+    var c:R0, n0:nat :| bigOfrom(c, n0, f, g);  
+    assert forall n:nat :: 0 <= n0 <= n ==> f(n) <= c*g(n);
+    
+    // we show that c'=a*c and n0'=n0
+    assert forall n:nat :: 0 <= n0 <= n ==> a*f(n) <= (a*c)*g(n);
+    assert bigOfrom(a*c, n0, n => a*f(n), g);
+  }
+
+  // If f1 ∈ O(g1) and f2 ∈ O(g2) then f1+f2 ∈ O(g1+g2)
+  lemma lem_bigO_sum(f1:nat->R0, g1:nat->R0, f2:nat->R0, g2:nat->R0)  
+    requires bigO(f1, g1) 
+    requires bigO(f2, g2) 
+    ensures  bigO(n => f1(n)+f2(n), n => g1(n)+g2(n)) 
+  {  
+    var c1:R0, n1:nat :| bigOfrom(c1, n1, f1, g1);  
+    assert forall n:nat :: 0 <= n1 <= n ==> f1(n) <= c1*g1(n);
+    var c2:R0, n2:nat :| bigOfrom(c2, n2, f2, g2);  
+    assert forall n:nat :: 0 <= n2 <= n ==> f2(n) <= c2*g2(n);   
+    
+    // we show that c=c1+c2 and n0=n1+n2
+    assert forall n:nat :: 0 <= n1+n2 <= n ==> f1(n) + f2(n) <= c1*g1(n) + c2*g2(n);
+    assert forall n:nat :: 0 <= n1+n2 <= n ==> f1(n) + f2(n) <= (c1+c2)*(g1(n) + g2(n));
+    assert bigOfrom(c1+c2, n1+n2, n => f1(n)+f2(n), n => g1(n)+g2(n));
+  }
+
+  // If f1 ∈ O(g1) and f2 ∈ O(g2) then f1*f2 ∈ O(g1*g2)
+  lemma lem_bigO_prod(f1:nat->R0, g1:nat->R0, f2:nat->R0, g2:nat->R0)  
+    requires bigO(f1, g1) 
+    requires bigO(f2, g2) 
+    ensures  bigO(n => f1(n)*f2(n), n => g1(n)*g2(n)) 
+  {  
+    var c1:R0, n1:nat :| bigOfrom(c1, n1, f1, g1);  
+    assert forall n:nat :: 0 <= n1 <= n ==> f1(n) <= c1*g1(n);
+    var c2:R0, n2:nat :| bigOfrom(c2, n2, f2, g2);  
+    assert forall n:nat :: 0 <= n2 <= n ==> f2(n) <= c2*g2(n);   
+    
+    // we show that c=c1*c2 and n0=n1+n2
+    assert forall n:nat :: 0 <= n1+n2 <= n ==> f1(n)*f2(n) <= (c1*g1(n))*(c2*g2(n));
+    assert forall n:nat :: 0 <= n1+n2 <= n ==> f1(n)*f2(n) <= (c1*c2)*(g1(n)*g2(n));
+    assert bigOfrom(c1*c2, n1+n2, n => f1(n)*f2(n), n => g1(n)*g2(n));
+  }
+
+  // Transitivity
+  // If f ∈ O(g) and g ∈ O(h) then f ∈ O(h)
+  lemma lem_bigO_trans(f:nat->R0, g:nat->R0, h:nat->R0)  
+    requires bigO(f, g) 
+    requires bigO(g, h) 
+    ensures  bigO(f, h) 
+  {  
+    var c1:R0, n1:nat :| bigOfrom(c1, n1, f, g);  
+    assert forall n:nat :: 0 <= n1 <= n ==> f(n) <= c1*g(n);
+    var c2:R0, n2:nat :| bigOfrom(c2, n2, g, h);  
+    assert forall n:nat :: 0 <= n2 <= n ==> g(n) <= c2*h(n);   
+    
+    // we show that c=c1*c2 and n0=n1+n2
+    forall n:nat | 0 <= n1+n2 <= n
+      ensures f(n) <= c1*c2*h(n)
+    {
+      if 0 <= n1+n2 <= n {
+        calc {
+             f(n); 
+          <= c1*g(n);
+          <= { assert g(n) <= c2*h(n); } 
+             c1*c2*h(n);         
+        }
+      }
+    }
+    assert bigOfrom(c1*c2, n1+n2, f, h);
+  }
+
+  // TODO: prove If f ∈ O(g) then f+g ∈ O(g)
+
+  /* Common growth rates comparison */
+
+  // log2(n) ∈ O(n) 
+  lemma {:axiom} lem_bigO_logBigOlin()
+    ensures bigO(logGrowth(), linGrowth()) 
+
+  // log2(n+1) ∈ O(n) 
+  lemma {:axiom} lem_bigO_logBigOlinV2()
+    ensures bigO(logGrowth2(), linGrowth())
+
+  // n ∈ O(n^2) 
+  lemma {:axiom} lem_bigO_linBigOquad()
+    ensures bigO(linGrowth(), quadGrowth()) 
+
+  // n^2 ∈ O(2^n)  
+  lemma {:axiom} lem_bigO_quadBigOexp()
+    ensures bigO(quadGrowth(), expGrowth())
+
+  // n ∈ O(2^n)  
+  lemma {:axiom} lem_bigO_linBigOexp()
+    ensures bigO(linGrowth(), expGrowth()) 
+
+}
